src/NLustre/CoIndToIndexed.v
@@ -32,7 +32,7 @@ Module Type COINDTOINDEXED
        (Import Ord     : NLORDERED        Ids Op       CESyn Syn)
        (CESem          : CESEMANTICS      Ids Op OpAux CESyn     Str)
        (Indexed        : NLSEMANTICS      Ids Op OpAux CESyn Syn Str Ord CESem)
-       (CoInd          : NLSEMANTICSCOIND Ids Op OpAux CESyn Syn).
+       (CoInd          : NLSEMANTICSCOIND Ids Op OpAux CESyn Syn Ord).
 
   Section Global.
 
